AwsCryptographicMaterialProviders/dafny/AwsCryptographyKeyStoreAdmin/src/PrefixUtils.dfy
@@ -1,0 +1,59 @@
+// Copyright Amazon.com Inc. or its affiliates. All Rights Reserved.
+// SPDX-License-Identifier: Apache-2.0
+
+module {:options "/functionSyntax:4" } PrefixUtils {
+  // import opened Structure
+  
+  opaque function AddingPrefixToKeysOfMapDoesNotCreateCollisions(
+    nameonly prefix: string,
+    nameonly aMap: map<string, string>
+  ): (output: map<string, string>)
+    ensures forall k <- aMap
+      ::
+      && prefix + k in output
+      && output[prefix + k] == aMap[k]
+    {
+      // Dafny needs some help.
+      // Adding a fixed string
+      // will not make any of the keys collide.
+      // However, this leaks a lot of complexity.
+      // This is why the function is now opaque.
+      // Otherwise things timeout
+      assert forall k <- aMap.Keys
+        ::
+        k == (prefix + k)[|prefix|..];
+
+      map k <- aMap :: prefix + k := aMap[k]
+    }
+
+  // opaque function AddingPrefixToCustomEncryptionContextDoesNotImpactReserved(
+  //   input: map<string, string>
+  // ): (output: map<string, string>
+  //   requires input.Keys !! BRANCH_KEY_RESTRICTED_FIELD_NAMES
+  //   ensures output.Keys !! BRANCH_KEY_RESTRICTED_FIELD_NAMES
+  //   ensures forall k <- 
+    
+  // opaque function RemovingAPrefixFromAllKeysOfMapDoesNotCreateCollisions(
+  //   nameonly prefix: string,
+  //   nameonly aMap: map<string, string>
+  // ): (output: map<string, string>)
+  //   requires forall k <- aMap :: |prefix| < |k| && prefix < k
+  //   ensures forall k <- aMap
+  //   ::
+  //     && k in aMap
+  //     && k[|prefix| ..] in output
+  //     && output[k[|prefix| ..] ] == aMap[k]
+  //   {
+  //     // Dafny needs some help.
+  //     // Adding a fixed string
+  //     // will not make any of the keys collide.
+  //     // However, this leaks a lot of complexity.
+  //     // This is why the function is now opaque.
+  //     // Otherwise things timeout
+  //     // assert forall k <- aMap.Keys
+  //     //   ::
+  //     //   k[|prefix|..] == (k - prefix);
+      
+  //     map k <- aMap :: k[|prefix| ..] := aMap[k]
+  //   }
+}
